SystemF/LocallyClosed.lean
@@ -35,16 +35,27 @@ inductive LcTm : Tm → Prop where
 
 /-
   All bound *term* indices in `t` are strictly less than `k`.
-  Note: it ignores bound type variables, so `LcAtTm 0` is not equivalent to `LcTm` as
-  we would expect.
+  Note: it ignores bound type variables, so `LcAtTm 0` is not equivalent to `LcTm`.
 -/
 inductive LcAtTm : ℕ → Tm → Prop where
   | bvar i k : i < k → LcAtTm k (#v i)
   | fvar x k : LcAtTm k ($v x)
   | app t₁ t₂ k : LcAtTm k t₁ → LcAtTm k t₂ → LcAtTm k (t₁ ◦ t₂)
   | lam T t k : LcAtTm (k + 1) t → LcAtTm k (ƛ T => t)
-  | tApp t T k : LcAtTm k t → LcAtTm k (t ⦃T⦄)
+  | tApp t T k : LcAtTm k t → LcAtTm k (t⦃T⦄)
   | tLam t k : LcAtTm k t → LcAtTm k (Λ' t)
+
+/-
+  All bound *type* indices inside the term `t` are strictly less than `k`.
+  Note: it ignores bound term variables, so `LcAtTyTm 0` is not equivalent to `LcTm`.
+-/
+inductive LcAtTyTm : ℕ → Tm → Prop where
+  | bvar i k : LcAtTyTm k (#v i)
+  | fvar X k : LcAtTyTm k ($v X)
+  | app t₁ t₂ k : LcAtTyTm k t₁ → LcAtTyTm k t₂ → LcAtTyTm k (t₁ ◦ t₂)
+  | lam T t k : LcAtTy k T → LcAtTyTm k t → LcAtTyTm k (ƛ T => t)
+  | tLam t k : LcAtTyTm (k + 1) t → LcAtTyTm k (Λ' t)
+  | tApp t T k : LcAtTyTm k t → LcAtTy k T → LcAtTyTm k (t⦃T⦄)
 
 -- Example: `∀. 0 -> 0` is a locally closed type
 example : LcTy (∀' (#T 0 ⇒ #T 0)) := by
@@ -511,6 +522,151 @@ theorem openTm_substTm_comm {t u v : Tm} {X : Name} {k : ℕ} (hu : LcTm u) :
     rw [ih]
   | tLam t ih =>
     simp only [substTm_tLam, openTm_tLam, Tm.tLam.injEq]
+    rw [ih]
+
+theorem openTm_substTm_comm_of_neq {t u : Tm} {x y : Name} {k : ℕ}
+    (hNeq : y ≠ x) (hu : LcTm u) :
+    (t[x ↦ u])⟪k, $vy⟫ = (t⟪k, $vy⟫)[x ↦ u] := by
+  rw [←openTm_substTm_comm hu]
+  simp [hNeq]
+
+theorem lcAtTyTm_openTmTy_id {t : Tm} {k : ℕ} (h : LcAtTyTm k t) (n : ℕ) (hn : k ≤ n) (V : Ty) :
+    t⟪n, V⟫ = t := by
+  induction h generalizing n with
+  | bvar i k => simp
+  | fvar X k => simp
+  | app t₁ t₂ k _ _ ih₁ ih₂ =>
+    simp only [openTmTy_app, Tm.app.injEq]
+    rw [ih₁ _ hn, ih₂ _ hn]
+    simp_all only [and_self]
+  | lam T t k h _ ih =>
+    simp only [openTmTy_lam, Tm.lam.injEq]
+    rw [ih _ (by omega)]
+    rw [lcAtTy_openTy_id h _ hn]
+    simp_all only [and_self]
+  | tLam t k _ ih =>
+    simp only [openTmTy_tLam, Tm.tLam.injEq]
+    rw [ih _ (by omega)]
+  | tApp t T k _ h ih =>
+    simp only [openTmTy_tApp, Tm.tApp.injEq]
+    rw [ih _ hn]
+    rw [lcAtTy_openTy_id h _ hn]
+    simp_all only [and_self]
+
+lemma lcAtTyTm_openTm_inv {t : Tm} {x : Name} {k n : ℕ}
+    (h : LcAtTyTm k (t⟪n, $vx⟫)) : LcAtTyTm k t := by
+  induction t generalizing k n with
+  | bvar idx => constructor
+  | fvar name => constructor
+  | app t₁ t₂ t₁_ih t₂_ih =>
+    cases h
+    constructor
+    · apply t₁_ih
+      assumption
+    · apply t₂_ih
+      assumption
+  | tApp t T ih =>
+    cases h
+    constructor
+    · apply ih
+      assumption
+    · assumption
+  | lam T t ih =>
+    cases h
+    constructor
+    · assumption
+    · apply ih
+      assumption
+  | tLam t ih =>
+    cases h
+    constructor
+    apply ih
+    assumption
+
+lemma lcAtTyTm_of_openTmTy {t : Tm} {X : Name} {k : ℕ}
+    (h : LcAtTyTm k (t⟪k, $TX⟫)) : LcAtTyTm (k + 1) t := by
+  induction t generalizing k with
+  | bvar idx => constructor
+  | fvar name => constructor
+  | app t₁ t₂ t₁_ih t₂_ih =>
+    cases h
+    constructor
+    · apply t₁_ih
+      assumption
+    · apply t₂_ih
+      assumption
+  | tApp t T ih =>
+    cases h
+    constructor
+    · apply ih
+      assumption
+    · apply lcAtTy_of_openTy
+      assumption
+  | lam T t ih =>
+    cases h
+    constructor
+    · apply lcAtTy_of_openTy
+      assumption
+    · apply ih
+      assumption
+  | tLam t ih =>
+    cases h
+    constructor
+    apply ih
+    assumption
+
+lemma lcTm_implies_lcAtTyTm0 {t : Tm} (h : LcTm t) : LcAtTyTm 0 t := by
+  induction h with
+  | fvar x => constructor
+  | app t₁ t₂ _ _ _ _ => constructor <;> assumption
+  | lam L T t _ _ ih =>
+    constructor
+    · apply lcTy_implies_lcAtTy0
+      assumption
+    · have ⟨x, hx⟩ := exists_fresh_name L
+      specialize ih x hx
+      apply lcAtTyTm_openTm_inv
+      assumption
+  | tApp t T _ _ ih =>
+    constructor
+    · apply ih
+    · apply lcTy_implies_lcAtTy0
+      assumption
+  | tLam L t _ ih =>
+    constructor
+    have ⟨X, hX⟩ := exists_fresh_name L
+    specialize ih X hX
+    apply lcAtTyTm_of_openTmTy
+    assumption
+
+@[simp]
+theorem openTmTy_lcTm_id {u : Tm} (hu : LcTm u) (k : ℕ) (V : Ty) :
+    u⟪k, V⟫ = u := by
+  apply lcAtTyTm_openTmTy_id
+  · apply lcTm_implies_lcAtTyTm0 hu
+  · simp only [zero_le]
+
+theorem openTmTy_substTm_comm {t u : Tm} {x : Name} {V : Ty} {k : ℕ} (hu : LcTm u) :
+    (t⟪k, V⟫)[x ↦ u] = (t[x ↦ u])⟪k, V⟫ := by
+  induction t generalizing k with
+  | bvar idx => simp
+  | fvar name =>
+    simp only [openTmTy_fvar, substTm_fvar, beq_iff_eq]
+    split
+    · rw [openTmTy_lcTm_id hu]
+    · simp
+  | app t₁ t₂ t₁_ih t₂_ih =>
+    simp only [openTmTy_app, substTm_app, Tm.app.injEq]
+    rw [t₁_ih, t₂_ih]
+    simp_all only [and_self]
+  | tApp t T ih =>
+    simp only [openTmTy_tApp, substTm_tApp, Tm.tApp.injEq, and_true]
+    rw [ih]
+  | lam T t ih =>
+    simp only [openTmTy_lam, substTm_lam, Tm.lam.injEq, true_and]
+    rw [ih]
+  | tLam t ih =>
+    simp only [openTmTy_tLam, substTm_tLam, Tm.tLam.injEq]
     rw [ih]
 
 end SystemF
