SystemF/Metatheory.lean
@@ -12,17 +12,16 @@ theorem typing_weakening {Γ₁ Γ₂ : Context} {t : Tm} {T U : Ty} {x : Name}
     (Γ₁ ++ (x, U) :: Γ₂) ⊢ t ∶ T := by
   generalize h : Γ₁ ++ Γ₂ = Γ at hTyping
   induction hTyping generalizing Γ₁ with
-  | var Γ x T _ _ =>
-    constructor
-    · aesop
-    · assumption
+  | var Γ x T _ _ _ =>
+    subst h
+    constructor <;> aesop
   | lam L Γ T₁ T₂ t _ _ ih =>
     let ctx := (Γ₁ ++ (x, U) :: Γ₂)
-    apply HasType.lam (L ∪ ctx.fv)
+    apply HasType.lam (L ∪ ctx.dom)
     · assumption
     · intro y hy
       have hy₁ : y ∉ L := by aesop
-      have hy₂ : y ∉ ctx.fv := by aesop
+      have hy₂ : y ∉ ctx.dom := by aesop
       have hWf_new : WfContext ((y, T₁) :: ctx) := by
         constructor <;> assumption
       simp only [ctx] at hWf_new
@@ -53,7 +52,7 @@ theorem typing_weakening {Γ₁ Γ₂ : Context} {t : Tm} {T U : Ty} {x : Name}
   For `x : T` in `Γ`, substituting free variable `X` with `U` in `Γ`
   yields `(x, T[X ↦ U])` in `Γ[X ↦ U]`.
 -/
-theorem subst_lookup {Γ : Context} {x : Name} {T U : Ty} {X : Name}
+theorem substCtx_lookup {Γ : Context} {x : Name} {T U : Ty} {X : Name}
     (h : (x, T) ∈ Γ) :
     (x, T[X ↦ U]) ∈ Γ[X ↦ U] := by
   induction Γ with
@@ -69,15 +68,40 @@ theorem subst_lookup {Γ : Context} {x : Name} {T U : Ty} {X : Name}
       cases head
       simp_all only [substCtx_cons, List.mem_cons, Prod.mk.injEq, or_true]
 
+@[simp]
+lemma substCtx_dom {Γ : Context} {X : Name} {U : Ty} :
+    (Γ[X ↦ U]).dom = Γ.dom := by
+  induction Γ with
+  | nil => simp
+  | cons head tail ih =>
+    cases head
+    simp only [substCtx_cons, dom_cons, Finset.singleton_union]
+    rw [ih]
 
+lemma substCtx_wf {Γ : Context} {X : Name} {U : Ty}
+    (hWf : WfContext Γ) (hU : LcTy U) : WfContext (Γ[X ↦ U]) := by
+  induction hWf with
+  | nil => simp; constructor
+  | cons Γ x T _ _ hLc ih =>
+    simp only [substCtx_cons]
+    constructor
+    · assumption
+    · simp only [substCtx_dom]
+      assumption
+    · exact substTy_lcTy hLc hU
+
+/-
+  Substitution lemma for types
+-/
 theorem typing_subst_ty {Γ : Context} {t : Tm} {T U : Ty} {X : Name}
     (hTyping : Γ ⊢ t ∶ T)
     (hLcTy : LcTy U) :
     (Γ[X ↦ U]) ⊢ (t[X ↦ U]) ∶ (T[X ↦ U]) := by
   induction hTyping with
-  | var Γ x T h₁ h₂ =>
+  | var Γ x T hWf h₁ h₂ =>
     constructor
-    · apply subst_lookup h₁
+    · exact substCtx_wf hWf hLcTy
+    · exact substCtx_lookup h₁
     · exact substTy_lcTy h₂ hLcTy
   | lam L Γ T₁ T₂ t h₁ h₂ ih =>
     apply HasType.lam (L ∪ {X} ∪ U.fv)
@@ -113,5 +137,71 @@ theorem typing_subst_ty {Γ : Context} {t : Tm} {T U : Ty} {X : Name}
     · simp only [subst_all] at ih
       exact ih
     · apply substTy_lcTy <;> assumption
+
+theorem typing_subst_tm {Γ₁ Γ₂ : Context} {t u : Tm} {T U : Ty} {x : Name}
+    (hTyping : (Γ₁ ++ (x, U) :: Γ₂) ⊢ t ∶ T)
+    (hSubstTyping : (Γ₁ ++ Γ₂) ⊢ u ∶ U) :
+    (Γ₁ ++ Γ₂) ⊢ (t[x ↦ u]) ∶ T := by
+  generalize h : Γ₁ ++ (x, U) :: Γ₂ = Γ at hTyping
+  induction hTyping generalizing Γ₁ with
+  | var Γ x' T _ _ _ =>
+    simp only [substTm_fvar, beq_iff_eq]
+    split
+    · simp_all only
+      rename_i hWf mem _ _
+      subst h
+      have : T = U := wf_lookup_mid hWf mem
+      rw [this]
+      assumption
+    · subst h
+      constructor
+      · exact typing_regularity_wf hSubstTyping
+      · aesop
+      · assumption
+  | lam L Γ T₁ T₂ t _ _ ih =>
+    simp only [substTm_lam]
+    apply HasType.lam (L ∪ {x} ∪ (Context.dom Γ))
+    · assumption
+    · intro y hy
+      have hLCu : LcTm u := typing_regularity_tm hSubstTyping
+      have hy₁ : y ∉ L := by aesop
+      have hy₂ : y ≠ x := by aesop
+      have hy₃ : y ∉ Context.dom (Γ₁ ++ Γ₂) := by aesop
+      rw [openTm_substTm_comm_of_neq hy₂ hLCu]
+      have : ((y, T₁) :: Γ₁ ++ Γ₂) ⊢ u ∶ U := by
+        have := typing_weakening (Γ₁ := []) (Γ₂ := Γ₁ ++ Γ₂) (x := y) (U := T₁) hSubstTyping
+        simp only [List.nil_append] at this
+        apply this
+        constructor
+        · exact typing_regularity_wf hSubstTyping
+        · exact hy₃
+        · assumption
+      -- Γ₁ ++ (x, U) :: Γ₂ = (y, T₁) :: (Γ₁ ++ (x, U) :: Γ₂)
+      exact @ih y hy₁ ((y, T₁) :: Γ₁) this (by aesop)
+  | app Γ t₁ t₂ T₁ T₂ _ _ ih₁ ih₂ =>
+    subst h
+    simp only [substTm_app]
+    constructor
+    · apply ih₁
+      · assumption
+      · rfl
+    · apply ih₂
+      · assumption
+      · rfl
+  | tLam L Γ t T _ ih =>
+    simp only [substTm_tLam]
+    apply HasType.tLam (L ∪ {x} ∪ (Context.fv Γ))
+    intro Y hY
+    have hLCu : LcTm u := typing_regularity_tm hSubstTyping
+    have hY₁ : Y ∉ L := by aesop
+    rw [←openTmTy_substTm_comm hLCu]
+    apply ih
+    · assumption
+    · assumption
+    · aesop
+  | tApp Γ t T₁ T₂ _ _ ih =>
+    constructor
+    apply ih <;> assumption
+    assumption
 
 end SystemF
